fix point_inv

specs/ecc/Spec.EC.Projective.Lemmas.fst
@@ -85,6 +85,116 @@ let ecdsa_verify_avoid_finv k p r =
 
 //-----------------------------------------
 
+val lemma_abc_is_zero (n:pos) (a b c:int) : Lemma
+  (requires c = 0)
+  (ensures  (a * b % n) * c % n = 0)
+
+let lemma_abc_is_zero n a b c =
+  calc (==) {
+    (a * b % n) * c % n;
+    (==) { }
+    (a * b % n) * 0 % n;
+    (==) { Math.Lemmas.lemma_mod_mul_distr_l (a * b) 0 n }
+    (a * b) * 0 % n;
+    (==) { Math.Lemmas.paren_mul_right a b 0; Math.Lemmas.mul_zero_right_is_zero b }
+    a * 0 % n;
+    (==) { Math.Lemmas.mul_zero_right_is_zero a; Math.Lemmas.small_mod 0 n }
+    0;
+   };
+  assert ((a * b % n) * c % n = 0)
+
+
+let point_inv_is_point_at_inf k p =
+  let ( +% ) = fadd k in
+  let ( *% ) = fmul k in
+  let (x, y, z) = p in
+
+  assert (point_inv k p);
+  assert (z = 0);
+  lemma_abc_is_zero k.prime y y z;
+  assert (y *% y *% z = 0);
+
+  lemma_abc_is_zero k.prime z z z;
+  assert (z *% z *% z = 0);
+  assert (k.coeff_b *% (z *% z *% z) = 0);
+
+  lemma_abc_is_zero k.prime k.coeff_a x (z *% z);
+  assert (k.coeff_a *% x *% (z *% z) = 0);
+  assert (x *% x *% x +% k.coeff_a *% x *% (z *% z) +% k.coeff_b *% (z *% z *% z) ==
+    x *% x *% x +% k.coeff_a *% x *% (z *% z) +% 0);
+  Math.Lemmas.small_mod (x *% x *% x +% k.coeff_a *% x *% (z *% z)) k.prime;
+  assert (x *% x *% x +% k.coeff_a *% x *% (z *% z) +% k.coeff_b *% (z *% z *% z) ==
+    x *% x *% x +% 0);
+  Math.Lemmas.small_mod (x *% x *% x) k.prime;
+  assert (0 == x *% x *% x);
+
+  k.prime_lemma ();
+  Lib.NatMod.lemma_mul_mod_prime_zero #k.prime (x *% x) x;
+  assert ((x *% x) % k.prime = 0 \/ x % k.prime = 0);
+  Math.Lemmas.small_mod x k.prime;
+  Math.Lemmas.small_mod (x *% x) k.prime;
+  Lib.NatMod.lemma_mul_mod_prime_zero #k.prime x x;
+  assert (x = 0)
+
+
+let lemma_is_point_at_inf k p =
+  let x, y, z = p in
+  let px, py = to_aff_point k p in
+  let zinv = finv k 0 in
+  assert (px == fmul k x zinv /\ py == fmul k y zinv);
+  assert (zinv == M.pow_mod #prime 0 (prime - 2));
+  M.lemma_pow_mod #prime 0 (prime - 2);
+  assert (zinv == M.pow 0 (prime - 2) % prime);
+  assert (prime > 2);
+  M.lemma_pow_zero (prime - 2);
+  Math.Lemmas.small_mod 0 k.prime;
+  assert (zinv == 0);
+  assert (px == 0 /\ py == 0)
+
+
+val point_inv_ec_lemma1: k:curve -> p:proj_point k -> Lemma
+  (requires point_inv k p /\ not (is_point_at_inf k p))
+  (ensures  is_on_curve k (to_aff_point k p))
+
+let point_inv_ec_lemma1 k p =
+  let ( +% ) = fadd k in
+  let ( *% ) = fmul k in
+  let ( /% ) a b = fmul k a (finv k b) in
+  let (x, y, z) = p in
+  assert (y *% y *% z = x *% x *% x +% k.coeff_a *% x *% (z *% z) +% k.coeff_b *% (z *% z *% z));
+  let px = x /% z in
+  let py = y /% z in
+  assert (z <> 0);
+  assume (py *% py = px *% px *% px +% k.coeff_a *% px +% k.coeff_b);
+  assert (is_on_curve k (px, py))
+
+
+val point_inv_ec_lemma2: k:curve -> p:proj_point k -> Lemma
+  (requires is_on_curve k (to_aff_point k p) /\ not (is_point_at_inf k p))
+  (ensures  point_inv k p)
+
+let point_inv_ec_lemma2 k p =
+  let ( +% ) = fadd k in
+  let ( *% ) = fmul k in
+  let ( /% ) a b = fmul k a (finv k b) in
+  let (x, y, z) = p in
+  let px = x /% z in
+  let py = y /% z in
+  assert (py *% py = px *% px *% px +% k.coeff_a *% px +% k.coeff_b);
+  assert (z <> 0);
+  assume (y *% y *% z = x *% x *% x +% k.coeff_a *% x *% (z *% z) +% k.coeff_b *% (z *% z *% z))
+
+
+let point_inv_ec_lemma k p =
+  Classical.move_requires (point_inv_ec_lemma1 k) p;
+  Classical.move_requires (point_inv_ec_lemma2 k) p
+
+
+let point_inv_lemma k p =
+  if is_point_at_inf k p then ()
+  else point_inv_ec_lemma k p
+
+
 let lemma_aff_is_point_at_inf k p =
   k.prime_lemma ();
   let (px, py, pz) = p in
@@ -92,22 +202,16 @@ let lemma_aff_is_point_at_inf k p =
   M.lemma_div_mod_prime_is_zero #prime py pz
 
 
-let lemma_aff_is_point_at_inf_c k p =
+val lemma_aff_is_point_at_inf_to_aff: k:curve -> p:proj_point k{point_inv_to_aff k p} ->
+  Lemma (let px, py, pz = p in is_aff_point_at_inf k (to_aff_point k p) == (pz = 0))
+
+let lemma_aff_is_point_at_inf_to_aff k p =
   lemma_aff_is_point_at_inf k p
 
 
-let to_aff_point_at_infinity_lemma k =
-  let px, py = to_aff_point k (point_at_inf k) in
-  assert (point_at_inf k = (0, 1, 0));
-  let zinv = finv k 0 in
-  assert (px == fmul k 0 zinv /\ py == fmul k 1 zinv);
-  assert (zinv == M.pow_mod #prime 0 (prime - 2));
-  M.lemma_pow_mod #prime 0 (prime - 2);
-  assert (zinv == M.pow 0 (prime - 2) % prime);
-  assert (prime > 2);
-  M.lemma_pow_zero (prime - 2);
-  assert (zinv == 0);
-  assert (px == 0 /\ py == 0)
+let lemma_aff_is_point_at_inf_c k p =
+  point_inv_lemma k p;
+  lemma_aff_is_point_at_inf_to_aff k p
 
 
 let lemma_proj_aff_id k p =
@@ -116,13 +220,52 @@ let lemma_proj_aff_id k p =
   let (rx, ry) = to_aff_point k (pX, pY, pZ) in
 
   if is_aff_point_at_inf k p then
-    to_aff_point_at_infinity_lemma k
+    lemma_is_point_at_inf k (point_at_inf k)
   else begin
     assert (pX = px /\ pY = pY /\ pZ = 1);
     assert (rx = fmul k pX (finv k pZ) /\ ry = fmul k pY (finv k pZ));
     M.lemma_div_mod_prime_one #prime pX;
     M.lemma_div_mod_prime_one #prime pY;
     assert (rx = pX /\ ry = pY) end
+
+//----------------
+
+let lemma_point_at_inf_c k =
+  let ( +% ) = fadd k in
+  let ( *% ) = fmul k in
+  let (x, y, z) = point_at_inf k in
+  assert (x = 0 && z = 0 && y = 1);
+  lemma_abc_is_zero k.prime y y z;
+  assert (y *% y *% z = 0);
+  lemma_abc_is_zero k.prime x x x;
+  assert (x *% x *% x = 0);
+  lemma_abc_is_zero k.prime k.coeff_a x (z *% z);
+  lemma_abc_is_zero k.prime z z z;
+  assert (y *% y *% z =
+    x *% x *% x +% k.coeff_a *% x *% (z *% z) +% k.coeff_b *% (z *% z *% z))
+
+
+let lemma_to_aff_point_c k p =
+  if is_point_at_inf k p then
+    lemma_is_point_at_inf k p
+  else point_inv_ec_lemma k p
+
+
+let lemma_to_proj_point_c k p =
+  let px, py = p in
+  if is_aff_point_at_inf k p then begin
+    assert (to_proj_point k p = point_at_inf k);
+    lemma_point_at_inf_c k end
+  else begin
+    k.prime_lemma ();
+    Lib.NatMod.lemma_div_mod_prime_one #k.prime px;
+    Lib.NatMod.lemma_div_mod_prime_one #k.prime py;
+    point_inv_ec_lemma k (to_proj_point k p) end
+
+//-----------------
+
+let to_aff_point_at_infinity_lemma k =
+  lemma_is_point_at_inf k (point_at_inf k)
 
 
 let to_aff_point_negate_lemma k p =
@@ -143,10 +286,17 @@ let to_aff_point_negate_lemma k p =
     (- (py * pz_inv) % k.prime) % k.prime; // (- py /% pz) % prime;
   };
   assert (to_aff_point k (point_negate k p) == aff_point_negate k (to_aff_point k p));
-  if is_point_at_inf k p then assert (pz = 0)
+
+  if is_point_at_inf k p then begin
+    assert (pz = 0);
+    assert (point_inv k (point_negate k p)) end
   else begin
-    Spec.EC.Lemmas.aff_point_negate_on_curve_lemma k (to_aff_point_c k p);
-    assert (is_on_curve k (to_aff_point k (point_negate k p))) end
+    point_inv_ec_lemma k p;
+    Spec.EC.Lemmas.aff_point_negate_on_curve_lemma k (to_aff_point k p);
+    assert (is_on_curve k (aff_point_negate k (to_aff_point k p)));
+    assert (is_on_curve k (to_aff_point k (point_negate k p)));
+    point_inv_ec_lemma k (point_negate k p);
+    assert (point_inv k (point_negate k p)) end
 
 
 let to_aff_point_add_lemma_a3 k p q = admit()
